$$\phi$$

$$V(\mu)=\mu$$

$$V(\mu)=\mu^2$$

$$V(\mu)=\mu^3$$

$$4\pi(d/2)^2=\pi d^2$$

$$\log y \propto \log \pi + 2 \log d$$

$$\mathcal{P}\big(y;\alpha,\beta\big)=\dfrac{y^{\alpha-1}\exp(-y/\beta)}{\Gamma(\alpha)\beta^{\alpha}}$$

$$y > 0, \alpha > 0$$

$$\mathrm{E}\lbrack y\rbrack=\alpha \beta$$

$$\mathrm{var}\lbrack y \rbrack = \alpha \beta^2$$

$$\Gamma(n)=(n-1)!$$

$$\mathcal{P}\big(y;\mu,\phi\big)=\Bigg(\frac{y}{\phi \mu} \Bigg)^{1/\phi}\frac{1}{y}\exp\Bigg(-\frac{y}{\phi\mu}\Bigg)\frac{1}{\Gamma(1/\phi)}$$

$$y > 0, \mu > 0, \phi > 0$$

$$\alpha=\frac{1}{\phi}, \beta=\mu\phi$$

$$\log(\mathrm{group} \thickspace \mathrm{variance}) \propto 2 \log(\mathrm{group} \thickspace \mathrm{mean})$$

$$V(\mu) \approx \mu^2$$

$$d(y;\mu)=2\Big \lbrace -\log \frac{y}{\mu} + \frac{y-\mu}{\mu}\Big \rbrace$$


$$D(y;\mu)=\sum_{i=1}^n w_i d(y_i, \mu_i) \sim \chi_{n-p'}^2$$


$$\phi \leq 1/3$$

$$\eta = \frac{1}{\mu}$$

$$\frac{r}{\lambda^2}$$

$$\mathcal{P}(y;\mu,\phi)=\Big(2\pi y^3 \phi\Big)^{-1/2}\exp \Big \lbrace - \frac{1}{2\phi} \frac{(y-\mu)^2}{y\mu^2} \Big \rbrace$$

$$\eta=\mu^{-2}$$

$$d(y, \mu)=\frac{(y-\mu)^2}{y\mu^2}$$

$$D(y, \hat{\mu})=\sum_{i=1}^n w_i d(y, \hat{\mu}_i)$$

$$\chi_1^2$$

$$D(y, \hat{\mu}) \sim \chi_{n-p'}^2$$

$$\delta$$

$$\psi(x)=\Gamma(x)'/\Gamma(x)$$

$$D(y, \hat{\mu})=-2\sum_{i=1}^n w_i \log \phi - w_i \log w_i + w_i \psi (w_i/\phi)$$

$$\bar{\phi}=\frac{1}{n-p'}\sum_{i=1}^n \frac{w_i (y_i - \hat{\mu}_i)^2}{\hat{\mu}_i^2}$$

$$\tilde{\phi}=\frac{D(y, \hat{\mu})}{n-p'}$$

$$\hat{\phi}=\frac{D(y, \hat{\mu})}{n}$$

$$\bar{\phi}=\frac{1}{n-p'}\sum_{i=1}^n \frac{w_i (y_i - \hat{\mu}_i)^2}{\hat{\mu}_i^3}$$


$$\mathrm{E}\lbrack z \rbrack = \frac{1}{\beta_2 + \beta_0 x + \beta_1 x^2}$$

$$y=xz$$

$$\mu = \mathrm{E} \lbrack y \rbrack = x \mathrm{E} \lbrack z \rbrack = \frac{x}{\beta_2 + \beta_0 x + \beta_1 x^2}$$

$$\frac{1}{\mu} = \beta_0 + \beta_1 x + \beta_2 \Bigg( \frac{1}{x} \Bigg)=\eta$$

$$\mathrm{E} \lbrack z \rbrack \rightarrow 0$$

$$x \rightarrow \infty$$

$$\mu \rightarrow 0$$

$$x \rightarrow 0$$

$$w_i=1$$

$$D(y, \hat{\mu}_i)=-2n\lbrace \log \phi + \psi(1/\phi)\rbrace$$

$$\psi_1(z)=d\psi(z)/dz$$

$$\sum_{i=1}^n(y_i - \hat{\mu}_i)/\hat{\mu}_i=0$$

$$\hat{\phi}=D(y, \hat{\mu})/n$$

$$\mu \rightarrow \infty$$

$$\mathcal{P}(y;\phi)=\frac{1}{\sqrt{2\pi\phi y^3}}\exp \Big\lbrace -\frac{1}{2y\phi}  \Big\rbrace$$